Launchbury/AbstractDenotational.thy
@@ -110,7 +110,7 @@ sublocale has_ESem ESem.
 abbreviation ESem_syn' ("\<lbrakk>_\<rbrakk>\<^bsub>_\<^esub>"  [60,60] 60) where "\<lbrakk>e\<rbrakk>\<^bsub>\<rho>\<^esub> \<equiv> ESem e \<cdot> \<rho>"
 abbreviation EvalHeapSem_syn'  ("\<^bold>\<lbrakk> _ \<^bold>\<rbrakk>\<^bsub>_\<^esub>"  [0,0] 110)  where "\<^bold>\<lbrakk>\<Gamma>\<^bold>\<rbrakk>\<^bsub>\<rho>\<^esub> \<equiv> evalHeap \<Gamma> (\<lambda> e. \<lbrakk>e\<rbrakk>\<^bsub>\<rho>\<^esub>)"
 abbreviation AHSem_syn ("\<lbrace>_\<rbrace>_"  [60,60] 60) where "\<lbrace>\<Gamma>\<rbrace>\<rho> \<equiv> HSem \<Gamma> \<cdot> \<rho>"
-abbreviation AHSem_fempty  ("\<lbrace>_\<rbrace>"  [60] 60) where "\<lbrace>\<Gamma>\<rbrace> \<equiv> \<lbrace>\<Gamma>\<rbrace>\<bottom>"
+abbreviation AHSem_bot ("\<lbrace>_\<rbrace>"  [60] 60) where "\<lbrace>\<Gamma>\<rbrace> \<equiv> \<lbrace>\<Gamma>\<rbrace>\<bottom>"
 
 subsubsection {* Equivariance of the semantics *}
 
